\begin{lemma}[Any constraint is satisfiable]
    \label{lemma:constraint-sat}
    Suppose that $[[Θ ⊢ SC]]$ then there exists 
    $[[uσ]]$ such that $[[(Θ  ⊢  SC) ⊢ uσ]]$.
\end{lemma}
\begin{proof}
    Let us define $[[uσ]]$
    on $[[dom(SC)]]$ in the following way: 
    $$
    [[ [uσ]α̂± ]] = 
    \begin{cases}
        [[iP]] & \text{if $[[(α̂± :≈ iP)]] \in [[SC]]$} \\
        [[iP]] & \text{if $[[(α̂± :≥ iP)]] \in [[SC]]$} \\
        [[iN]] & \text{if $[[(α̂± :≈ iN)]] \in [[SC]]$} \\
    \end{cases}
    $$
    Then $[[(Θ  ⊢  SC) ⊢ uσ]]$ follows immediately
    from the reflexivity of equivalence and subtyping
    (\cref{lemma:subtyping-reflexivity}) and the corresponding
    rules 
    \ruleref{\ottdruleSATSCEPEqLabel}, 
    \ruleref{\ottdruleSATSCENEqLabel},
    and \ruleref{\ottdruleSATSCESupLabel}.
\end{proof}


\begin{lemma}[Constraint Entry Satiisfaction is Stable under Equivalence]
    \label{lemma:entry-sat-equiv}
    \begin{itemize}
        \item [$-$] If $[[Γ ⊢ iN1 : scE]]$ and $[[Γ ⊢ iN1 ≈ iN2]]$ then $[[Γ ⊢ iN2 : scE]]$.
        \item [$+$] If $[[Γ ⊢ iP1 : scE]]$ and $[[Γ ⊢ iP1 ≈ iP2]]$ then $[[Γ ⊢ iP2 : scE]]$.
    \end{itemize}
\end{lemma}
\begin{proof}
    \begin{itemize}
        \item [$-$] Then $[[scE]]$ has form $[[(α̂⁻ :≈ iM)]]$, 
            and by inversion, $[[Γ ⊢ iN1 ≈ iM]]$.
            Then by transitivity, $[[Γ ⊢ iN2 ≈ iM]]$, 
            meaning $[[Γ ⊢ iN2 : scE]]$.
        \item [$+$] Let us consider what form $[[scE]]$ has.
            \begin{caseof}
                \item $[[scE]] = [[(α̂⁺ :≈ iQ)]]$. Then $[[Γ ⊢ iP1 ≈ iQ]]$,
                    and hence, $[[Γ ⊢ iP2 ≈ iQ]]$ by transitivity.
                    Then $[[Γ ⊢ iP2 : scE]]$.
                \item $[[scE]] = [[(α̂⁺ :≥ iQ)]]$. Then $[[Γ ⊢ iP1 ≥ iQ]]$,
                    and hence, $[[Γ ⊢ iP2 ≥ iQ]]$ by transitivity.
                    Then $[[Γ ⊢ iP2 : scE]]$.
            \end{caseof}
    \end{itemize}
\end{proof}

\begin{corollary}[Constraint Satisfaction is stable under Equivalence]
    \label{corollary:sat-equiv}
    \hfill\\
    If $[[(Θ  ⊢  SC) ⊢ uσ1]]$ and $[[Θ|dom(SC) ⊢ uσ1 ≈ uσ2]]$ then $[[(Θ  ⊢  SC) ⊢ uσ2]]$;\\
    if $[[(Θ  ⊢  UC) ⊢ uσ1]]$ and $[[Θ|dom(SC) ⊢ uσ1 ≈ uσ2]]$ then $[[(Θ  ⊢  UC) ⊢ uσ2]]$.
\end{corollary}

\begin{corollary}[Normalization preserves Constraint Satisfaction]
    \label{corollary:nf-sat}
    \hfill\\
    If $[[(Θ  ⊢  SC) ⊢ uσ]]$ then $(Θ  ⊢ SC) ⊢ nf(uσ)$;\\
    if $[[(Θ  ⊢  UC) ⊢ uσ]]$ then $(Θ  ⊢ UC) ⊢ nf(uσ)$.
\end{corollary}



