\begin{observation} [Least Upper Bound algorithm is deterministic]
  \label{obs:lub-deterministic}
  For types $[[Γ ⊢ iP1]]$, and $[[Γ ⊢ iP2]]$,
  if $[[Γ ⊨ iP1 ∨ iP2 = iQ]]$ and $[[Γ ⊨ iP1 ∨ iP2 = iQ']]$
  then $[[iQ = iQ']]$.
\end{observation}
\begin{proof}
  The shape of $[[iP1]]$ and $[[iP2]]$ uniquely determines the rule 
  applied to infer the upper bound.
  By looking at the inference rules,
  it is easy to see that the result of the least upper bound algorithm depends on 
  \begin{itemize}
    \item the inputs of the algorithm (that is $[[iP1]]$, $[[iP2]]$, and $[[Γ]]$),
      which are fixed;
    \item the result of the anti-unification algorithm
      applied to normalized input, which is deterministic
      by \cref{obs:au-deterministic}; 
    \item the result of the recursive call, which is deterministic by the induction hypothesis.
  \end{itemize}
\end{proof}

\begin{lemma}[Characterization of the Supertypes]
  \label{lemma:shape-of-supertypes}
  Let us define the
  set of upper bounds of a positive type $\UB([[iP]])$ in the following way:

  \hfill

  \begin{tabular}{@{}lr@{}} \toprule
    % supertypes of ... & ... are \\ 
    $[[G ⊢ iP]]$          & $\UB([[G ⊢ iP]])$ \\ \midrule
    \addlinespace[0.7em]
    $[[ G ⊢ pb ]]$        & $\{[[ ∃nas.pb ]] \ \mid \ \text{for }[[nas]]\}$ \\
    \addlinespace[0.7em]
    $[[ G ⊢ ∃nbs.iQ ]]$   & %$\Set{ [[iQ]] \ | \begin{array}{l} [[iQ]] \in \UB([[iP]]) \\  \text{ s.t. } [[fv iQ ∩ {nbs} = ∅]] \end{array}}$  \\
                            $\UB([[G, nbs ⊢ iQ]])$ not using $[[nbs]]$ \\
    \addlinespace[0.7em]
    $[[ G ⊢ ↓iM ]]$       & $\Set{ [[ ∃nas.↓iM' ]] \ | \begin{array}{l}
                                                         \text{for $[[nas]]$, $[[iM']]$, and $[[iNs]]$ s.t. }\\
                                                         \text{$[[G ⊢ iNi]]$, $[[G,nas ⊢ iM']]$,  and $[[ [iNs/nas] ↓iM' ≈ ↓iM ]]$}
                                                       \end{array}}$  \\
  \end{tabular}

  Then $\UB([[G ⊢ iP]]) \equiv \{[[iQ]]\ \mid \ [[G ⊢ iQ ≥ iP]] \}$.
\end{lemma}
\begin{proof}
  By induction on $[[G ⊢ iP]]$.
  \begin{caseof}
  \item $[[iP]] = [[pb]]$\\
    Immediately from \cref{lemma:var-subt}
  \item $[[iP = ∃nbs.iP']]$\\
    Then if $[[G ⊢ iQ ≥ ∃nbs.iP']]$, then by
    \cref{lemma:quant-rule-decomposition}, $[[G, nbs ⊢ iQ ≥ iP']]$, 
    and $[[fv iQ ∩ {nbs} = ∅]]$ by the convention. The other
    direction holds by \ruleref{\ottdruleDOneExistsLabel}. This way,
    $\{[[iQ]] \mid [[G ⊢ iQ ≥ ∃nbs.iP']] \} = \{[[iQ]] \mid  [[G, nbs ⊢ iQ
    ≥ iP']] \text{ s.t. } [[fv(iQ) ∩ {nbs} = ∅]] \}$. From the induction
    hypothesis, the latter is equal to $\UB([[G, nbs ⊢ iP']])$ not using
    $[[nbs]]$, i.e. $\UB([[G ⊢ ∃nbs.iP']])$.
  \item $[[iP = ↓iM]]$\\
    Then let us consider two subcases upper bounds without outer quantifiers (we
    denote the corresponding set restriction as $|_{\not\exists}$) and upper
    bounds with outer quantifiers ($|_{\exists}$). We prove that for both of
    these groups, the restricted sets are equal.
    % ∃a.P(f a) <=> ∃b∊Im(f).P(b)

    \begin{caseof}
      \item \label{case:sup-shape-down-zero}
      $[[iQ]] \neq [[∃nbs.iQ']]$\\
      Then the last applied rule to infer
      $[[G ⊢ iQ ≥ ↓iM]]$ must be \ruleref{\ottdruleDOneShiftDLabel},
      which means $[[iQ]] = [[↓iM']]$, and by inversion, $[[G ⊢ iM' ≈ iM]]$,
      then by \cref{lemma:equiv-completeness} and
      \ruleref{\ottdruleEOneShiftDLabel}, $[[↓iM' ≈ ↓iM]]$.
      This way, $[[iQ]] = [[↓iM']] \in \{ [[↓iM']] \mid [[↓iM' ≈ ↓iM]] \} = \UB([[Γ⊢↓iM]])|_{\not\exists}$.

      In the other direction,
      $
      \begin{aligned}[t]
        [[↓iM' ≈ ↓iM]] &\Rightarrow [[G ⊢ ↓iM' ≈ ↓iM]]
                       && \text{by \cref{lemma:equiv-soundness}, since
                          $[[G ⊢ ↓iM']]$ by \cref{lemma:wf-equiv} }\\
                       &\Rightarrow [[G ⊢ ↓iM' ≥ ↓iM]]
                       && \text{by inversion}
      \end{aligned}
      $
      \item $[[iQ]] = [[∃nbs.iQ']]$ (for non-empty $[[nbs]]$)\\
        Then the last rule applied to infer $[[G ⊢ ∃nbs.iQ' ≥ ↓iM]]$
        must be \ruleref{\ottdruleDOneExistsLabel}.
        Inversion of this rule gives us $[[G ⊢ [iNs/nbs]iQ' ≥ ↓iM]]$
        for some $[[G ⊢ iNi]]$. Notice that $[[ [iNs/nbs]iQ' ]]$ has no outer
        quantifiers. Thus from \cref{case:sup-shape-down-zero},
        $[[ [iNs/nbs]iQ' ≈ ↓iM ]]$, which is only possible if $[[iQ']] = [[↓iM']]$.
        This way, $[[iQ]] = [[∃nbs.↓iM']] \in \UB([[Γ⊢↓iM]])|_{\exists}$ (notice
        that $[[nbs]]$ is not empty).

        In the other direction,
        $
        \begin{aligned}[t]
          [[ [iNs/nbs]↓iM' ≈ ↓iM]] &\Rightarrow [[G ⊢ [iNs/nbs] ↓iM' ≈ ↓iM]]
          && \text{by \cref{lemma:equiv-soundness}, since
             $[[G ⊢ [iNs/nbs] ↓iM']]$ by \cref{lemma:wf-equiv} }\\
                                  &\Rightarrow [[G ⊢ [iNs/nbs]↓iM' ≥ ↓iM]]
         && \text{by inversion}\\
                                  &\Rightarrow [[G ⊢ ∃nbs.↓iM' ≥ ↓iM]] 
         && \text{by \ruleref{\ottdruleDOneExistsLabel}}\\
        \end{aligned}
        $
    \end{caseof}
    
  \end{caseof}
\end{proof}

\begin{lemma}[Characterization of the Normalized Supertypes]
  \label{lemma:shape-supertypes-norm}
  For a normalized positive type $[[iP = nf(iP)]]$,
  let us define the set of normalized upper bounds in the following way:
  
  \hfill

  \begin{tabular}{@{}lr@{}} \toprule
    % supertypes of ... & ... are \\ 
    $[[G ⊢ iP]]$          & $\NFUB([[G ⊢ iP]])$ \\ \midrule
    \addlinespace[0.7em]
    $[[ G ⊢ pb ]]$        & $\{ [[pb]] \}$ \\
    \addlinespace[0.7em]
    $[[ G ⊢ ∃nbs.iP ]]$   & %$\Set{ [[iQ]] \ | \begin{array}{l} [[iQ]] \in \UB([[iP]]) \\  \text{ s.t. } [[fv iQ ∩ {nbs} = ∅]] \end{array}}$  \\
    $\NFUB([[G, nbs ⊢ iP]])$ not using $[[nbs]]$ \\
    \addlinespace[0.7em]
    $[[ G ⊢ ↓iM ]]$       & $\Set{ [[ ∃nas.↓iM' ]] \ | \begin{array}{l}
                                                         \text{for $[[nas]]$, $[[iM']]$, and $[[iNs]]$ s.t. $[[ord {nas} in iM' = nas]]$,}\\
                                                         \text{$[[G ⊢ iNi]]$, $[[G,nas ⊢ iM']]$,  and $[[ [iNs/nas] ↓iM' = ↓iM ]]$}
                                                       \end{array}}$  \\
  \end{tabular}

  Then $\NFUB([[G ⊢ iP]]) \equiv \{[[nf(iQ)]]\ \mid \ [[G ⊢ iQ ≥ iP]] \}$.
\end{lemma}


\begin{proof}
  By induction on $[[G ⊢ iP]]$.
  \begin{caseof}
  \item $[[iP]] = [[pb]]$\\
    Then from \cref{lemma:shape-of-supertypes},
    $\{[[nf(iQ)]]\ \mid \ [[G ⊢ iQ ≥ pb]] \} = \{[[ nf(∃nas.pb) ]] \ \mid \
    \text{for some }[[nas]]\}  = \{[[pb]]\}$ 
  \item $[[iP = ∃nbs.iP']]$\\
    $
    \begin{aligned}[t]
      \NFUB([[Γ ⊢ ∃nbs.iP']]) &= \NFUB([[Γ, nbs ⊢ iP']]) \text{ not using $[[nbs]]$}\\
                              &= \{ [[nf(iQ)]] \mid [[Γ, nbs ⊢ iQ ≥ iP']]  \}
                                \text{ not using $[[nbs]]$}
                              && \text{by the induction hypothesis}\\
                              &= \{ [[nf(iQ)]] \mid [[Γ, nbs ⊢ iQ ≥ iP']]
                                \text{ s.t. $[[fv iQ]] \cap [[nbs]] = \emptyset$}
                                \}
                             && \text{because $[[fv nf(iQ)]] = [[fv iQ]]$ by \cref{lemma:fv-nf}}\\
                              &= \{ [[nf(iQ)]] \mid [[iQ]] \in \UB([[Γ, nbs ⊢ iP']]) \text{ s.t. $[[fv iQ]] \cap [[nbs]] = \emptyset$}
                                \}
                            && \text{by \cref{lemma:shape-of-supertypes}}\\
                              &= \{ [[nf(iQ)]] \mid [[iQ]] \in \UB([[Γ ⊢ ∃nbs.iP']])
                                \}
                              && \text{by the definition of $\UB{}$}\\
                              &= \{ [[nf(iQ)]] \mid [[Γ ⊢ iQ ≥ ∃nbs.iP']]
                                \}
                              && \text{by \cref{lemma:shape-of-supertypes}}\\
    \end{aligned}
    $
  
  \item $[[iP = ↓iM]]$ Let us prove the set equality by two inclusions.
  \begin{itemize}
    \item [$\subseteq$]
      Suppose that $[[Γ ⊢ iQ ≥ ↓iM]]$ and $[[iM]]$ is normalized.

      By \cref{lemma:shape-of-supertypes},
      $[[iQ]] \in \UB([[Γ ⊢ ↓iM]])$.
      Then by definition of $\UB{}$,
      $[[iQ = ∃nas.↓iM']]$ 
      for some $[[nas]]$, $[[iM']]$, and $[[Γ ⊢ σ :{nas}]]$ s.t.  
      $[[ [σ] ↓iM' ≈ ↓iM ]]$.

      We need to show that $[[nf(iQ)]] \in \NFUB([[Γ ⊢ ↓iM]])$.
      Notice that $[[nf(iQ)]] = [[nf(∃nas.↓iM')]] = [[∃nas0.↓iM0]]$, 
      where $[[nf(iM') = iM0]]$ and $[[ord {nas} in iM0 = nas0]]$.

      The belonging of $[[∃nas0.↓iM0]]$ to $\NFUB([[Γ ⊢ ↓iM]])$ means that
      \begin{enumerate}
        \item $[[ord {nas0} in iM0 = nas0]]$ and
        \item that there exists $[[Γ ⊢ σ0 :{nas0}]]$ such that 
          $[[ [σ0] ↓iM0 = ↓iM ]]$.
      \end{enumerate}
      The first requirement holds by \cref{corollary:ord-idemp}.
      To show the second requirement, we construct
      $[[σ0]]$ as $[[nf(σ|fv iM')]]$.
      Let us show the required properties of $[[σ0]]$:
      \begin{enumerate}
        \item $[[Γ ⊢ σ0 :{nas0}]]$. 
          Notice that by \cref{lemma:subst-restr-sig},
          $[[Γ ⊢ σ|fv(iM') :  {nas} ∩ fv(iM')]]$, 
          which we rewrite as 
          $[[Γ ⊢ σ|fv(iM') :{nas0}]]$ 
          (since by \cref{lemma:ord-soundness}
          $[[{nas0} = {nas} ∩ fv iM0]]$ as sets, 
          and $[[fv(iM0) = fv(iM')]]$ by \cref{lemma:fv-nf}).
          Then by \cref{lemma:norm-subst-sig}, 
          $[[Γ ⊢ nf(σ|fv(iM')) :{nas0}]]$,
          that is $[[Γ ⊢ σ0 :{nas0}]]$.
        \item $[[ [σ0] ↓iM0 = ↓iM ]]$.
          $[[ [σ] ↓iM' ≈ ↓iM ]]$ means 
          $[[ [σ|fv(iM')]↓iM' ≈ ↓iM ]]$ by 
          \cref{lemma:subst-restr-fv}.
          Then by \cref{lemma:decl-equiv-algorithmization}, 
          $[[ nf([σ|fv(iM')]↓iM') = nf(↓iM) ]]$, 
          implying $[[ [σ0] ↓iM0 = nf(↓iM) ]]$
          by \cref{lemma:norm-subst-distr},
          and further $[[ [σ0] ↓iM0 = ↓iM ]]$
          by \cref{lemma:norm-idemp} (since $[[↓iM]]$ is normal by assumption).
      \end{enumerate}
    
    \item [$\supseteq$]
      Suppose that a type belongs to $\NFUB([[Γ ⊢ ↓iM]])$ for a normalized 
      $[[↓iM]]$.
      Then it must have shape $[[∃nas0.↓iM0]]$ for some $[[nas0]]$, $[[iM0]]$,
      and $[[Γ ⊢ σ0 :{nas0}]]$ such that 
      $[[ ord {nas0} in iM0 = nas0 ]]$ and $[[ [σ0] ↓iM0 = ↓iM ]]$.
      It is suffices to show that 
      \begin{enumerate*}
        \item $[[∃nas0.↓iM0]]$ is normalized itself, and 
        \item $[[Γ ⊢ ∃nas0.↓iM0 ≥ ↓iM]]$.
      \end{enumerate*}

      \begin{enumerate}
        \item By definition, 
          $[[nf(∃nas0.↓iM0) = ∃nas1.↓iM1]]$, 
          where $[[iM1 = nf(iM0)]]$ and $[[ord {nas0} in iM1 = nas1]]$.
          First, notice that by 
          \cref{lemma:ord-completeness,lemma:normalization-soundness}, 
          $[[ord {nas0} in iM1]] = [[ord {nas0} in iM0]] = [[nas0]]$. 
          This way, $[[nf(∃nas0.↓iM0) = ∃nas0.↓nf(iM0)]]$.
          Second, $[[iM0]]$ is normalized by \cref{lemma:normal-after-subst}, 
          since $[[ [σ0] ↓iM0 = ↓iM ]]$ is normal. 
          As such, $[[nf(∃nas0.↓iM0) = ∃nas0.↓iM0]]$, 
          in other words, $[[∃nas0.↓iM0]]$ is normalized.
        \item $[[Γ ⊢ ∃nas0.↓iM0 ≥ ↓iM]]$ holds immediately by 
          \ruleref{\ottdruleDOneExistsLabel} with the substitution 
          $[[σ0]]$. Notice that $[[Γ ⊢ [σ0]↓iM0 ≥ ↓iM]]$
          follows from $[[ [σ0] ↓iM0 = ↓iM ]]$
          by reflexivity of subtyping (\cref{lemma:subtyping-reflexivity}).
      \end{enumerate}



    \end{itemize}
  \end{caseof}
\end{proof}

\begin{lemma}
  \label{observation:ub-context-irrelevant}
  Upper bounds of a type do not depend on the context
  as soon as the type is well-formed in it.

  If $[[Γ1 ⊢ iP]]$ and $[[Γ2 ⊢ iP]]$ then
  $\UB([[Γ1 ⊢ iP]]) = \UB([[Γ2 ⊢ iP]])$ and
  $\NFUB([[Γ1 ⊢ iP]]) = \NFUB([[Γ2 ⊢ iP]])$
\end{lemma}
\begin{proof}
  We prove both inclusions by structural induction on  
  $[[iP]]$.
  \begin{caseof}
    \item $[[iP]] = [[pb]]$
      Then $\UB([[Γ1 ⊢ pb]]) = \UB([[Γ2 ⊢ pb]]) = 
      \{[[∃nas.pb]] \mid \text{for some }[[nas]]\}$.
      $\NFUB([[Γ1 ⊢ pb]]) = \NFUB([[Γ2 ⊢ pb]]) = \{[[pb]]\}$.
    \item $[[iP]] = [[∃nbs.iP']]$.
      Then $\UB([[Γ1 ⊢ ∃nbs.iP']]) = \UB([[Γ1, nbs ⊢ iP']])$ not using $[[nbs]]$.
      $\UB([[Γ2 ⊢ ∃nbs.iP']]) = \UB([[Γ2, nbs ⊢ iP']])$ not using $[[nbs]]$.
      By the induction hypothesis, $\UB([[Γ1, nbs ⊢ iP']]) = \UB([[Γ2, nbs ⊢ iP']])$,
      and if we restrict these sets to the same domain, they stay equal.
      Analogously, $\NFUB([[Γ1 ⊢ ∃nbs.iP']]) = \NFUB([[Γ2 ⊢ ∃nbs.iP']])$.
    \item $[[iP]] = [[↓iM]]$.
      Suppose that $[[∃nas.↓iM']] \in \UB([[Γ1 ⊢ ↓iM]])$. It means that 
      $[[Γ1, nas ⊢ iM']]$ and there exist $[[Γ1 ⊢ iNs]]$ s.t. 
      $[[ [iNs/nas] ↓iM' ≈ ↓iM ]]$, or in other terms, 
      there exists $[[Γ1 ⊢ σ :{nas}]]$ such that $[[ [σ] ↓iM' ≈ ↓iM ]]$.

      We need to show that $[[∃nas.↓iM']] \in UB([[Γ2 ⊢ ↓iM]])$,  
      in other words, $[[Γ2, nas ⊢ iM']]$ and there exists
      $[[Γ2 ⊢ σ0 :{nas}]]$ such that $[[ [σ0] ↓iM' ≈ ↓iM ]]$.

      First, let us show $[[Γ2, nas ⊢ iM']]$. 
      Notice that $[[ [σ] ↓iM' ≈ ↓iM ]]$ implies $[[ fv([σ]iM') = fv(↓iM) ]]$ 
      by \cref{lemma:equiv-fv}. By \cref{lemma:subst-fv},
      $[[ fv(iM') \ {nas} ⊆ fv([σ]iM') ]]$. This way, 
      $[[ fv(iM') \ {nas} ⊆ fv(iM) ]]$,
      implying $[[ fv(iM') ⊆ fv(iM) ∪ {nas} ]]$.
      By \cref{lemma:wf-soundness}, $[[Γ2 ⊢ ↓iM]]$ implies $[[fv iM ⊆ Γ2]]$,
      hence, $[[fv iM' ⊆ (Γ2, nas)]]$, which by \cref{corollary:wf-ctxt-strengthening}
      means $[[Γ2, nas ⊢ iM']]$.
      
      Second, let us construct the required $[[σ0]]$ in the following way:
      $$
      \begin{cases}
          [[ [σ0]αi⁻ = [σ]αi⁻  ]] & \text{for $[[αi⁻ ∊ {nas} ∩ fv(iM')]]$ }\\
          [[ [σ0]αi⁻ = ∀γ⁺.↑γ⁺ ]] & \text{for $[[αi⁻ ∊ {nas} \ fv(iM')]]$ }\\
          [[ [σ0]γ±  = γ± ]]      & \text{for any other $[[γ±]]$ }\\
      \end{cases}
      $$
      This construction of a substitution coincides with 
      the one from the proof of \cref{lemma:subt-ctxt-irrelevance}.
      This way, for $[[σ0]]$, hold the same properties:
      \begin{enumerate}
        \item $[[ [σ0]iM' = [σ]iM' ]]$,
          which in particular, implies $[[ [σ0]↓iM = [σ]↓iM ]]$,
          and thus, $[[ [σ]↓iM' ≈ ↓iM ]]$ can be rewritten to
          $[[ [σ0]↓iM' ≈ ↓iM ]]$; and
        \item $[[  fv([σ]iM') ⊢ σ0 :{nas}]]$,
          which, as noted above, can be rewritten to 
          $[[  fv(iM) ⊢ σ0 :{nas}]]$,
          and since $[[fv iM ⊆ Γ2]]$, 
          weakened to $[[ Γ2 ⊢ σ0 :{nas}]]$.
      \end{enumerate}

      The proof of $\NFUB([[Γ1 ⊢ ↓iM]]) \subseteq \NFUB([[Γ2 ⊢ ↓iM]])$
      is analogous.
      The differences are:
      \begin{enumerate}
        \item $[[ord {nas} in iM' = nas]]$ holds by assumption, 
        \item $[[ [σ] ↓iM' = ↓iM ]]$ implies $[[ fv([σ]iM') = fv(↓iM) ]]$ by rewriting,
        \item $[[ [σ] ↓iM' = ↓iM ]]$ and $[[ [σ0]↓iM = [σ]↓iM ]]$
          imply $[[ [σ0] ↓iM' = ↓iM ]]$ by rewriting.
      \end{enumerate}
  \end{caseof}
\end{proof}

\begin{lemma}[Soundness of the Least Upper Bound]
  \label{lemma:lub-soundness}
  For types $[[Γ ⊢ iP1]]$, and $[[Γ ⊢ iP2]]$,
  if $[[Γ ⊨ iP1 ∨ iP2 = iQ]]$ then
  \begin{enumerate}
    \item[(i)]  $[[Γ ⊢ iQ]]$
    \item[(ii)] $[[Γ ⊢ iQ ≥ iP1]]$ and $[[Γ ⊢ iQ ≥ iP2]]$
  \end{enumerate}
\end{lemma}
\begin{proof}
  Induction on $[[Γ ⊨ iP1 ∨ iP2 = iQ]]$.
  \begin{caseof}
  \item $[[Γ ⊨ pa ∨ pa = pa]]$\\
     Then $[[Γ ⊢ pa]]$ by assumption, and
     $[[Γ ⊢ pa ≥ pa]]$ by \ruleref{\ottdruleDOnePVarLabel}.
   \item $[[Γ ⊨ ∃nas.iP1 ∨ ∃nbs.iP2 = iQ]]$\\
     Then by inversion of $[[Γ ⊢ ∃nas.iPi]]$  and
     weakening, $[[Γ, {nas}, {nbs} ⊢ iPi]]$, hence, the induction
     hypothesis applies to $[[Γ, {nas}, {nbs} ⊨ iP1 ∨ iP2 = iQ]]$. Then
     \begin{itemize}
       \item[(i)] $[[Γ, {nas}, {nbs} ⊢ iQ]]$,
       \item[(ii)] $[[Γ, {nas}, {nbs} ⊢ iQ ≥ iP1]]$,
       \item[(iii)] $[[Γ, {nas}, {nbs} ⊢ iQ ≥ iP2]]$.
     \end{itemize}

     To prove $[[Γ ⊢ iQ]]$, it suffices to show that
     $[[fv(iQ) ∩ (Γ, {nas}, {nbs})]] = [[fv(iQ) ∩ Γ]]$ (and then apply \cref{lemma:wf-ctxt-equiv}).
     The inclusion right-to-left is self-evident. To show
     $[[fv(iQ) ∩ (Γ, {nas}, {nbs})]] \subseteq [[fv(iQ) ∩ Γ]]$, we prove that 
     $[[fv(iQ)]] \subseteq [[Γ]]$

     $
     \begin{aligned}[t]
       [[fv(iQ)]] &\subseteq [[fv iP1 ∩ fv iP2]]
                  && \text{by \cref{lemma:fv-propagation}}\\
                  &\subseteq [[((Γ, nas) \ {nbs}) ∩ ((Γ, nbs) \ {nas})]]
                  &&
                  \begin{array}{l}
                  \text{since $[[Γ ⊢ ∃nas.iP1]]$,~ $[[fv(iP1)]]
                  \subseteq [[(Γ, nas)]] = [[(Γ, nas)
                  \ {nbs}]]$}\\
                  \text{(the latter is because by the Barendregt's
                  convention,}\\
                    \text{$[[(Γ, nas) ∩ {nbs} = ∅]]$);
                    similarly, $[[fv(iP2)]] \subseteq [[(Γ, nbs) \ {nas}]]$}\\
                  \end{array}\\
                  &\subseteq [[Γ]]
     \end{aligned}
     $

     To show $[[Γ ⊢ iQ ≥ ∃nas.iP1]]$, we apply
     \ruleref{\ottdruleDOneExistsLabel}.
     Then $[[Γ, nas ⊢ iQ ≥ iP1]]$ holds since
     $[[Γ, {nas}, {nbs} ⊢ iQ ≥ iP1]]$ (by the induction hypothesis),
     $[[Γ, nas ⊢ iQ]]$ (by weakening), and $[[Γ, nas ⊢ iP1]]$.

     Judgment $[[Γ ⊢ iQ ≥ ∃nbs.iP2]]$ is proved symmetrically.
  \item $[[Γ ⊨ ↓iN ∨ ↓iM = ∃nas.[nas / ToList Ξ]uP]]$.
    By the inversion, $[[G,· ⊨ nf(↓iN) ≈au nf(↓iM) ⫤ (Ξ, uP, aus1, aus2)]]$.
    Then by the soundness of anti-unification (\cref{lemma:au-soundness}),
    \begin{enumerate}
    \item[(i)] $[[Γ ; Ξ ⊢ uP]]$, then
      by \cref{lemma:var-dealgo-wf},
      \begin{equation} \label{fact:nas-uP-is-wf} [[Γ, nas ⊢ [nas / ToList Ξ]uP]] \end{equation}
    \item[(ii)] $[[Γ ; · ⊢ aus1 : Ξ]]$ and $[[Γ ; · ⊢ aus2 : Ξ]]$.
      Assuming that $[[Ξ]] = [[nub1,..,nubn]]$,
      the antiunification solutions $[[aus1]]$ and $[[aus2]]$ can be
      put explicitly as $[[aus1]] = [[(nub1 :≈ iN1,..,nubn :≈ iNn)]]$,
      and $[[aus2]] = [[(nub1 :≈ iM1,..,nubn :≈ iMn)]]$.
      Then
      \begin{equation}
        \label{fact:aus1-is-compose}
        [[ aus1 ]] = [[ (iNs / nas) ○ (nas / ToList Ξ) ]] 
      \end{equation}
      \begin{equation}
        \label{fact:aus2-is-compose}
        [[ aus2 ]] = [[ (iMs / nas) ○ (nas / ToList Ξ) ]]
      \end{equation}
    \end{enumerate}
  \item[(iii)] $[[ [aus1] uQ = iP1 ]]$ and $[[ [aus2] uQ = iP1 ]]$,
    which, by \ref{fact:aus1-is-compose} and \ref{fact:aus2-is-compose},
    means
    \begin{equation}
      \label{fact:sub-sub-uP-iN}
      [[ [iNs / nas][nas / ToList Ξ]uP = nf(↓iN) ]]
    \end{equation}
    \begin{equation}
      \label{fact:sub-sub-uP-iM}
      [[ [iMs / nas][nas / ToList Ξ]uP = nf(↓iM) ]]
    \end{equation}

    Then $[[Γ ⊢ ∃nas.[nas / ToList Ξ]uP]]$
    follows directly from \ref{fact:nas-uP-is-wf}.

    To show $[[Γ ⊢ ∃nas.[nas / ToList Ξ]uP ≥ ↓iN]]$,
    we apply \ruleref{\ottdruleDOneExistsLabel},
    instantiating $[[nas]]$ with $[[iNs]]$.
    Then $[[Γ ⊢ [iNs / nas][nas / ToList Ξ]uP ≥ ↓iN ]]$ follows
    from \ref{fact:sub-sub-uP-iN} and 
    since $[[Γ ⊢ nf(↓iN) ≥ ↓iN]]$ (by \cref{corollary:nf-sound-wrt-subt-equiv}).

    Analogously, instantiating $[[nas]]$ with $[[iMs]]$,
    gives us $[[Γ ⊢ [iMs / nas][nas / ToList Ξ]uP ≥ ↓iM ]]$
    (from \ref{fact:sub-sub-uP-iM}), and hence,
    $[[Γ ⊢ ∃nas.[nas / ToList Ξ]uP ≥ ↓iM]]$.

  \end{caseof}

\end{proof}


\begin{lemma}[Completeness and Initiality of the Least Upper Bound]
  \label{lemma:lub-completeness}
  For types $[[Γ ⊢ iP1]]$, $[[Γ ⊢ iP2]]$, and $[[Γ ⊢ iQ]]$
  such that $[[Γ ⊢ iQ ≥ iP1]]$ and $[[Γ ⊢ iQ ≥ iP2]]$,
  there exists $[[iQ']]$ s.t. $[[Γ ⊨ iP1 ∨ iP2 = iQ']]$ 
  and $[[Γ ⊢ iQ ≥ iQ']]$.
\end{lemma}

\begin{proof}
  Induction on the pair $([[iP1]], [[iP2]])$.
  From \cref{lemma:shape-supertypes-norm},
  $[[iQ]] \in \UB([[Γ ⊢ iP1]]) \cap \UB([[Γ ⊢ iP2]])$.
  Let us consider the cases of what $[[iP1]]$ and $[[iP2]]$ are (i.e. the last
  rules to infer $[[Γ ⊢ iPi]]$).
  \begin{caseof}
    \item $[[iP1]] = [[∃nbs1.iQ1]]$, $[[iP2]] = [[∃nbs2.iQ2]]$, where either
      $[[nbs1]]$ or $[[nbs2]]$ is not empty\\
      \label{case:ub-completeness-exists}

      Then
      $
      \begin{aligned}[t]
        [[iQ]] &\in         \UB([[Γ ⊢ ∃nbs1.iQ1]]) \cap \UB([[Γ ⊢ ∃nbs2.iQ2]]) \\
              & \subseteq  \UB([[Γ, nbs1 ⊢ iQ1]]) \cap \UB([[Γ, nbs2 ⊢ iQ2]])
              && \text{from the definition of $\UB{}$}\\
              & =  \UB([[Γ, {nbs1}, {nbs2} ⊢ iQ1]]) \cap \UB([[Γ, {nbs1}, {nbs2} ⊢ iQ2]])
              && \text{by \cref{observation:ub-context-irrelevant}, weakening and
                  exchange}\\
              & = \{[[iQ']]\ \mid \ [[Γ, {nbs1}, {nbs2}  ⊢ iQ' ≥ iQ1]] \} \cap
                  \{[[iQ']]\ \mid \ [[Γ, {nbs1}, {nbs2}  ⊢ iQ' ≥ iQ2]] \}
              && \text{by \cref{lemma:shape-of-supertypes},}\\
      \end{aligned}
      $\\
      meaning that $[[Γ, {nbs1}, {nbs2} ⊢ iQ ≥ iQ1]]$ and $[[Γ, {nbs1}, {nbs2} ⊢ iQ ≥
      iQ2]]$. Then the next step of the algorithm---the recursive call 
      $[[Γ, {nbs1}, {nbs2} ⊨ iQ1 ∨ iQ2 = iQ']]$
      terminates by the induction hypothesis, 
      and moreover, $[[ Γ, {nbs1}, {nbs2} ⊢ iQ ≥ iQ' ]]$.
      This way, the result of the algorithm is $[[iQ']]$, i.e.
      $[[Γ ⊨ iP1 ∨ iP2 = iQ']]$.

      Since both $[[iQ]]$ and $[[iQ']]$ are sound upper bounds,
      $[[Γ ⊢ iQ]]$ and $[[Γ ⊢ iQ']]$, and therefore,
      $[[ Γ, {nbs1}, {nbs2} ⊢ iQ ≥ iQ' ]]$ can be strengthened to
      $[[ Γ ⊢ iQ ≥ iQ' ]]$ by \cref{lemma:subt-ctxt-irrelevance}.

    \item $[[iP1]] = [[pa]]$ and $[[iP2]] = [[↓iN]]$\\
      \label{case:ub-completeness-unmatching}
      Then the set of common upper bounds of $[[↓iN]]$ and $[[pa]]$
      is empty, and thus, $[[iQ]] \in \UB([[Γ ⊢ iP1]]) \cap \UB([[Γ ⊢ iP2]])$
      gives a contradiction:\\
      $
      \begin{aligned}[t]
        [[iQ]] &\in         \UB([[Γ ⊢ pa]]) \cap \UB([[Γ ⊢ ↓iN]]) \\
              & = \{[[∃nas.pa]]\  \mid \cdots \} \cap
                  \{[[∃nbs.↓iM']]\ \mid \cdots \}
              && \text{by the definition of $\UB{}$}\\
              & = \emptyset
              && \text{since $[[pa]] \neq [[↓iM']]$ for any $[[iM']]$}\\
      \end{aligned}
      $
    \item $[[iP1]] = [[↓iN]]$ and $[[iP2]] = [[pa]]$\\
      Symmetric to \cref{case:ub-completeness-unmatching}

    \item $[[iP1]] = [[pa]]$ and $[[iP2]] = [[pb]]$ (where $[[pb]] \neq [[pa]]$)\\
      Similarly to \cref{case:ub-completeness-unmatching},
      the set of common upper bounds is empty, which leads to the contradiction:

      $
      \begin{aligned}[t]
      [[iQ]] &\in         \UB([[Γ ⊢ pa]]) \cap \UB([[Γ ⊢ pb]]) \\
            & = \{[[∃nas.pa]]\  \mid \cdots \} \cap
                \{[[∃nbs.pb]]\ \mid \cdots \}
            && \text{by the definition of $\UB{}$}\\
            & = \emptyset
            && \text{since $[[pa]] \neq [[pb]]$}
      \end{aligned}
      $
    \item $[[iP1]] = [[pa]]$ and $[[iP2]] = [[pa]]$\\
      Then the algorithm terminates in one step (\ruleref{\ottdruleLUBVarLabel})
      and the result is $[[pa]]$, i.e. $[[G ⊨ pa ∨ pa = pa]]$.

      Since $[[iQ]] \in \UB([[Γ ⊢ pa]])$,
      $[[iQ]] = [[∃nas.pa]]$.
      Then $[[Γ ⊢ ∃nas.pa ≥ pa]]$ by \ruleref{\ottdruleDOneExistsLabel}:
      $[[nas]]$ can be instantiated with arbitrary negative types (for example
      $[[∀β⁺.↑β⁺]]$), since the substitution for unused variables does not change the term
      $[[ [iNs/nas]pa]] = [[pa]]$,
      and then $[[Γ ⊢ pa ≥ pa]]$ by \ruleref{\ottdruleDOnePVarLabel}.

    \item $[[iP1]] = [[↓iM1]]$ and $[[iP2]] = [[↓iM2]]$ \label{case:ub-completeness-shift}\\
      Then on the next step, the algorithm tries to anti-unify $[[nf(↓iM1)]]$ and
      $[[nf(↓iM2)]]$. By \cref{lemma:au-completeness}, to show that the
      anti-unification algorithm terminates, it suffices to
      demonstrate that a sound anti-unification solution exists.

      Notice that

      $
      \begin{aligned}[t]
        [[nf(iQ)]] &\in \NFUB([[Γ ⊢ nf(↓iM1)]]) \cap \NFUB([[Γ ⊢ nf(↓iM2)]]) \\
              &= \NFUB([[Γ ⊢ ↓nf(iM1)]]) \cap \NFUB([[Γ ⊢ ↓nf(iM2)]]) \\
              &=           \begin{array}{l}
                              \Set{ [[ ∃nas.↓iM' ]] \ | \begin{array}{l}
                                                          \text{for $[[nas]]$, $[[iM']]$, and $[[iNs]]$ s.t. $[[ord {nas} in iM' = nas]]$,}\\
                                                          \text{$[[G ⊢ iNi]]$, $[[G,nas ⊢ iM']]$,  and $[[ [iNs/nas] ↓iM' = ↓nf(iM1) ]]$}
                                                        \end{array}}\\ \cap\\
                              \Set{ [[ ∃nas.↓iM' ]] \ | \begin{array}{l}
                                                          \text{for $[[nas]]$, $[[iM']]$, and $[[iNs]]$ s.t. $[[ord {nas} in iM' = nas]]$,}\\
                                                          \text{$[[G ⊢ iNs1]]$,
                                                          $[[G ⊢ iNs2]]$, $[[G,nas ⊢ iM']]$,  and $[[ [iNs/nas] ↓iM' = ↓nf(iM2) ]]$}
                                                        \end{array}}
                            \end{array}\\
                &=
                  \Set{ [[ ∃nas.↓iM' ]] \ | \begin{array}{l}
                                              \text{for $[[nas]]$, $[[iM']]$,
                                              $[[iNs1]]$ and $[[iNs2]]$ s.t. $[[ord {nas} in iM' = nas]]$,}\\
                                              \text{$[[G ⊢ iNs1]]$, $[[G ⊢ iNs2]]$, $[[G,nas ⊢ iM']]$,
                                              $[[ [iNs1/nas] ↓iM' = ↓nf(iM1)]]$, and
                                              $[[ [iNs2/nas] ↓iM' = ↓nf(iM2)]]$
                                              }
                                            \end{array}}\\
      \end{aligned}
      $\\
      The fact that the latter set is non-empty means that there exist $[[nas]],
      [[iM']]$, $[[iNs1]]$ and $[[iNs2]]$ such that
      \begin{enumerate}
      \item[(i)] $[[G,nas ⊢ iM']]$ (notice that $[[iM']]$ is normal)
      \item[(ii)] $[[G ⊢ iNs1]]$ and $[[G ⊢ iNs1]]$,
      \item[(iii)] $[[ [iNs1/nas] ↓iM' = ↓nf(iM1)]]$ and $[[ [iNs2/nas] ↓iM' = ↓nf(iM2)]]$
      \end{enumerate}

      For each negative variable $[[α⁻]]$ from $[[nas]]$, let us choose a
      fresh negative anti-unification variable $[[α̂⁻]]$, and denote the
      list of these variables as $[[nuas]]$.
      Let us show that $([[nuas]],~ [[ [nuas/nas]↓iM' ]],~ [[iNs1/nuas]],~ [[iNs2/nuas]])$ is a
      sound anti-unifier of $[[nf(↓iM1)]]$ and $[[nf(↓iM2)]]$ in context $[[Γ]]$:

      \begin{itemize}
        \item $[[nuas]]$ is negative by construction,
        \item $[[Γ ; {nuas} ⊢ [nuas/nas]↓iM']]$ because $[[Γ, nas ⊢ ↓iM']]$ 
        (\cref{lemma:var-algo-wf}),
        \item $[[Γ ; · ⊢ (iNs1/nuas) :{nuas}]]$ because $[[Γ ⊢ iNs1]]$ and
          $[[Γ ; · ⊢ (iNs2/nuas) :{nuas}]]$ because $[[Γ ⊢ iNs2]]$,
        \item $[[ [iNs1/nuas] [nuas/nas] ↓iM' ]] = [[ [iNs1/nas] ↓iM' ]] =
          [[↓nf(iM1)]] = [[nf(↓iM1)]]$.
        \item $[[ [iNs2/nuas] [nuas/nas] ↓iM' ]] = [[ [iNs2/nas] ↓iM' ]] = [[↓nf(iM2)]] = [[nf(↓iM2)]]$.
      \end{itemize}

      Then by the completeness of the anti-unification
      (\cref{lemma:au-completeness}), the anti-unification algorithm
      terminates, so is the Least Upper Bound algorithm invoking it, 
      i.e. $[[iQ']] = [[∃nbs.[nbs / ToList Ξ]uP]]$, where
      $[[(Ξ, uP, aus1, aus2)]]$ is the result of the anti-unification
      of $[[nf(↓iM1)]]$ and $[[nf(↓iM2)]]$ in context $[[Γ]]$.

      Moreover, \cref{lemma:au-completeness} also says that the found anti-unification 
      solution is initial, i.e. there exists $[[aus]]$ such that
      $[[Γ;Ξ ⊢ aus :{nuas}]]$ and $[[ [aus][nuas/nas]↓uM' = uP ]]$.

      Let $[[σ]]$ be a sequential Kleisli composition of the following
      substitutions:
      \begin{enumerate*}
      \item[(i)] $[[nuas/nas]]$,
      \item[(ii)] $[[aus]]$, and
      \item[(iii)] $[[nbs / ToList Ξ]]$.
      \end{enumerate*}
      Notice that $[[Γ, nbs ⊢ σ :{nas}]]$
      and $[[ [σ]↓uM' ]] = [[ [nbs / ToList Ξ][aus][nuas/nas]↓uM' ]] = [[ [nbs /
      ToList Ξ]uP ]]$. In particular, from the reflexivity of subtyping:
      $[[Γ, nbs ⊢ [σ]↓iM' ≥ [nbs / ToList Ξ]uP]]$.

      It allows us to show $[[Γ ⊢ nf(iQ) ≥ iQ']]$, i.e. $[[Γ ⊢ ∃nas.↓iM' ≥
      ∃nbs.[nbs / ToList Ξ]uP]]$, by applying \ruleref{\ottdruleDOneExistsLabel},
      instantiating $[[nas]]$ with respect to $[[σ]]$. Finally, $[[Γ ⊢ iQ ≥ iQ']]$
      by transitively combining $[[Γ ⊢ nf(iQ) ≥ iQ']]$ and $[[Γ ⊢ iQ ≥ nf(iQ)]]$ 
      (holds by \cref{corollary:nf-sound-wrt-subt-equiv} and inversion).
  \end{caseof}
\end{proof}