\begin{restatable}[Determinacy of typing algorithm]{lemma}{lemmaTypingDeterminacy}
    \label{lemma:typing-determinacy}
    Suppose that $[[Γ ⊢ Φ]]$ and $[[Γ ⊢ Θ]]$. Then 
    \begin{itemize}
        \item [$+$] If $[[Γ; Φ ⊨ v : iP]]$ and $[[Γ; Φ ⊨ v : iP']]$ then $[[iP = iP']]$.
        \item [$-$] If $[[Γ; Φ ⊨ c : iN]]$ and $[[Γ; Φ ⊨ c : iN']]$ then $[[iN = iN']]$.
        \item If $[[Γ; Φ; Θ ⊨ uN ● args ⇒> uM ⫤ Θ'; SC]]$ and 
            $[[Γ; Φ; Θ ⊨ uN ● args ⇒> uM' ⫤ Θ'; SC']]$ then 
            $[[uM = uM']]$, $[[Θ]] = [[Θ']]$, and $[[SC]] =[[SC']]$.  
    \end{itemize}
\end{restatable}

\begin{restatable}[Algorithmic Substitution Strengthening]{lemma}{lemmaSubstRestrUV}
    \label{lemma:subst-restr-uv}
    Restricting the substitution to the algorithmic 
    variables of the
    substitution subject does not affect the result.
    Suppose that $[[uσ]]$ is an algorithmic substitution,
    $[[uP]]$ and $[[uN]]$ are algorithmic types. Then
 \begin{itemize}
        \item[$+$] $[[ [uσ]uP ]] = [[ [uσ|uv uP]uP ]]$,
        \item[$-$] $[[ [uσ]uN ]] = [[ [uσ|uv uN]uN ]]$
    \end{itemize}
\end{restatable}

\begin{restatable}[Substitutions equal on the algorithmic variables]{lemma}{lemmaSubstEqAlgVar}
    \label{lemma:subst-eq-algovar}
    Suppose that $[[uσ1]]$ and $[[uσ2]]$ are 
    normalized substitutions of signature $[[Θ ⊢ uσi : Ξ]]$.
    Then 
    \begin{enumerate}
        \item [$+$] for a normalized type $[[Γ; Ξ ⊢ uP]]$, if $[[ [uσ1]uP = [uσ2]uP ]]$ then
            $[[uσ1|(uv uP)  = uσ2|(uv uP)]]$;
        \item [$-$] for a normalized type $[[Γ; Ξ ⊢ uN]]$, if $[[ [uσ1]uN = [uσ2]uN ]]$ then
            $[[uσ1|(uv uN)  = uσ2|(uv uN)]]$.
    \end{enumerate}
\end{restatable}


\begin{restatable}[Substitutions equivalent on the algorithmic variables]{corollary}{corollarySubstEquivAlgVar}
    \label{lemma:subst-equiv-algovar}
    Suppose that $[[uσ1]]$ and $[[uσ2]]$ are substitutions 
    of signature $[[Θ ⊢ uσi : Ξ]]$ where $[[Γ ⊢ Θ]]$.
    Then 
    \begin{enumerate}
        \item [$+$] for a type $[[Γ; Ξ ⊢ uP]]$, if $[[Γ ⊢ [uσ1]uP ≈ [uσ2]uP]]$ then
            $[[Θ ⊢ uσ1 ≈ uσ2 : uv uP]]$;
        \item [$-$] for a type $[[Γ; Ξ ⊢ uN]]$, if $[[Γ ⊢ [uσ1]uN ≈ [uσ2]uN]]$ then
            $[[Θ ⊢ uσ1 ≈ uσ2 : uv uN]]$.
    \end{enumerate}
\end{restatable}
